checkpoint

OtbnModel.v
@@ -2,6 +2,8 @@ Require Import Coq.Strings.String.
 Require Import Coq.Lists.List.
 Require Import Coq.micromega.Lia.
 Require Import Coq.ZArith.ZArith.
+Require Import coqutil.Semantics.OmniSmallstepCombinators.
+Require Coq.Strings.HexString.
 Import ListNotations.
 Local Open Scope Z_scope.
 
@@ -69,6 +71,7 @@ Section Flags.
   | FG1
   .
 
+  (* TODO: maybe make this a pair *)
   Inductive flag : Type :=
   | flagC : forall fg : flag_group, flag
   | flagM : forall fg : flag_group, flag
@@ -92,101 +95,286 @@ Section ISA.
   | rshift : Z -> shift
   .
 
+  (* Indirect register (may have increment bit set or not). *)
+  Inductive ind : Type :=
+  | ind_noinc : gpr -> ind
+  | ind_inc : gpr -> ind
+  .
+
   (* Straightline instructions (no control flow) *)
-  Inductive Insn : Type :=
-  | Mulqacc : forall (z : bool), limb -> limb -> Z -> Insn
-  | Mulqacc_wo : forall (z : bool), wdr -> limb -> limb -> Z -> Insn
-  | Mulqacc_so : forall (z : bool) (L : bool), wdr -> limb -> limb -> Z -> Insn
-  | Addm : wdr -> wdr -> wdr -> Insn
-  | Subm : wdr -> wdr -> wdr -> Insn
-  | Add : wdr -> wdr -> wdr -> shift -> flag_group -> Insn
-  | Addc : wdr -> wdr -> wdr -> shift -> flag_group -> Insn
-  | Sub : wdr -> wdr -> wdr -> shift -> flag_group -> Insn
-  | Subb : wdr -> wdr -> wdr -> shift -> flag_group -> Insn
-  | Rshi : wdr -> wdr -> wdr -> Z -> Insn
+  Inductive sinsn : Type :=
+  | Addi : gpr -> gpr -> Z -> sinsn
+  | Bn_mulqacc : forall (z : bool), limb -> limb -> Z -> sinsn
+  | Bn_mulqacc_wo : forall (z : bool), wdr -> limb -> limb -> Z -> sinsn
+  | Bn_mulqacc_so : forall (z : bool) (L : bool), wdr -> limb -> limb -> Z -> sinsn
+  | Bn_addm : wdr -> wdr -> wdr -> sinsn
+  | Bn_subm : wdr -> wdr -> wdr -> sinsn
+  | Bn_add : wdr -> wdr -> wdr -> shift -> flag_group -> sinsn
+  | Bn_addc : wdr -> wdr -> wdr -> shift -> flag_group -> sinsn
+  | Bn_sub : wdr -> wdr -> wdr -> shift -> flag_group -> sinsn
+  | Bn_subb : wdr -> wdr -> wdr -> shift -> flag_group -> sinsn
+  | Bn_rshi : wdr -> wdr -> wdr -> Z -> sinsn
+  | Bn_movr : ind -> ind -> sinsn
+  | Bn_lid : ind -> Z -> ind -> sinsn
+  .
+
+  (* Control-flow instructions *)
+  Inductive cinsn : Type :=
+  (* TODO: technically ret is a special case of JALR, but only RET is used in practice *)
+  | Ret : cinsn
+  | Ecall : cinsn
+  | Jal : gpr -> Z -> cinsn
+  | Bne : gpr -> gpr -> Z -> cinsn
+  | Beq : gpr -> gpr -> Z -> cinsn
+  | Loop : gpr -> Z -> cinsn
+  | Loopi : Z -> Z -> cinsn
+  .
+
+  Inductive insn : Type :=
+  | Straightline : sinsn -> insn
+  | Control : cinsn -> insn
   .
 
 End ISA.
 
 (* Notations to interpret assembly code. *)
-Module Notations.
+Module OtbnNotations.
   Coercion gpreg : gpr >-> reg.
   Coercion wdreg : wdr >-> reg.
   Coercion wsreg : wsr >-> reg.
-  Notation "x '.0'" := (limb0 x) (at level 0).
-  Notation "x '.1'" := (limb1 x) (at level 0).
-  Notation "x '.2'" := (limb2 x) (at level 0).
-  Notation "x '.3'" := (limb3 x) (at level 0).
-  Notation "'bn.mulqacc' a , b , imm" := (Mulqacc false a b imm) (at level 40).
-  Notation "'bn.mulqacc.z' a , b , imm" := (Mulqacc true a b imm) (at level 40).
-  Notation "'bn.mulqacc.wo' d , a , b , imm" := (Mulqacc_wo false d a b imm) (at level 40).
-  Notation "'bn.mulqacc.wo.z' d , a , b , imm" := (Mulqacc_wo true d a b imm) (at level 40).
-  Notation "'bn.mulqacc.so' d '.L' , a , b , imm" := (Mulqacc_so false true d a b imm) (at level 40).
-  Notation "'bn.mulqacc.so' d '.U' , a , b , imm" := (Mulqacc_so false false d a b imm) (at level 40).
-  Notation "'bn.mulqacc.so.z' d '.L' , a , b , imm" := (Mulqacc_so true true d a b imm) (at level 40).
-  Notation "'bn.mulqacc.so.z' d '.U' , a , b , imm" := (Mulqacc_so true false d a b imm) (at level 40).
-  Notation "'bn.addm' d , a , b " := (Addm d a b) (at level 40).
-  Notation "'bn.add' d , a , b '<<' s , fg" := (Add d a b (lshift s) fg) (at level 40).
-  Notation "'bn.add' d , a , b '>>' s , fg" := (Add d a b (rshift s) fg) (at level 40).
+  Coercion ind_noinc : gpr >-> ind.
+  Coercion Straightline : sinsn >-> insn. 
+  Coercion Control : cinsn >-> insn. 
+  Declare Scope otbn_scope.
+  Delimit Scope otbn_scope with otbn.
 
-  (*
-  (* Program graph with control flow. Block constructors are named
-     after the control-flow instruction they end with. *)
-  Inductive Block : Type :=
-  | Ret : list Insn -> Block
-  | Ecall : list Insn -> Block
-  (* Tail-call pattern: jal x0, foo *)
-  | JumpNoLink : list Insn -> string -> Block
-  (* Function call pattern: jal x1, foo *)
-  | Call : list Insn -> string -> Block -> Block
-  | Bne : list Insn -> gpr -> gpr -> string -> Block -> Block
-  | LoopEnd : list Insn -> Block (* loop start *) -> Block (* post-loop *) -> Block
+  Notation "x '.0'" := (limb0 x) (at level 0) : otbn_scope.
+  Notation "x '.1'" := (limb1 x) (at level 0) : otbn_scope.
+  Notation "x '.2'" := (limb2 x) (at level 0) : otbn_scope.
+  Notation "x '.3'" := (limb3 x) (at level 0) : otbn_scope.
+  Notation "a '++'" := (ind_inc a) (at level 20) : otbn_scope.
+  Notation "'addi' d , a , imm" := (Addi d a imm) (at level 40) : otbn_scope. 
+  Notation "'bn.mulqacc' a , b , imm" := (Bn_mulqacc false a b imm) (at level 40) : otbn_scope.
+  Notation "'bn.mulqacc.z' a , b , imm" := (Bn_mulqacc true a b imm) (at level 40) : otbn_scope.
+  Notation "'bn.mulqacc.wo' d , a , b , imm" := (Bn_mulqacc_wo false d a b imm) (at level 40) : otbn_scope.
+  Notation "'bn.mulqacc.wo.z' d , a , b , imm" := (Bn_mulqacc_wo true d a b imm) (at level 40) : otbn_scope.
+  Notation "'bn.mulqacc.so' d '.L' , a , b , imm" := (Bn_mulqacc_so false true d a b imm) (at level 40) : otbn_scope.
+  Notation "'bn.mulqacc.so' d '.U' , a , b , imm" := (Bn_mulqacc_so false false d a b imm) (at level 40) : otbn_scope.
+  Notation "'bn.mulqacc.so.z' d '.L' , a , b , imm" := (Bn_mulqacc_so true true d a b imm) (at level 40) : otbn_scope.
+  Notation "'bn.mulqacc.so.z' d '.U' , a , b , imm" := (Bn_mulqacc_so true false d a b imm) (at level 40) : otbn_scope.
+  Notation "'bn.addm' d , a , b " := (Bn_addm d a b) (at level 40) : otbn_scope.
+  Notation "'bn.subm' d , a , b " := (Bn_subm d a b) (at level 40) : otbn_scope.
+  Notation "'bn.add' d , a , b , fg" := (Bn_add d a b (lshift 0) fg) (at level 40) : otbn_scope.
+  Notation "'bn.add' d , a , b '<<' s , fg" := (Bn_add d a b (lshift s) fg) (at level 40) : otbn_scope.
+  Notation "'bn.add' d , a , b '>>' s , fg" := (Bn_add d a b (rshift s) fg) (at level 40) : otbn_scope.
+  Notation "'bn.addc' d , a , b , fg" := (Bn_addc d a b (lshift 0) fg) (at level 40) : otbn_scope.
+  Notation "'bn.addc' d , a , b '<<' s , fg" := (Bn_addc d a b (lshift s) fg) (at level 40) : otbn_scope.
+  Notation "'bn.addc' d , a , b '>>' s , fg" := (Bn_addc d a b (rshift s) fg) (at level 40) : otbn_scope.
+  Notation "'bn.sub' d , a , b , fg" := (Bn_sub d a b (lshift 0) fg) (at level 40) : otbn_scope.
+  Notation "'bn.sub' d , a , b '<<' s , fg" := (Bn_sub d a b (lshift s) fg) (at level 40) : otbn_scope.
+  Notation "'bn.sub' d , a , b '>>' s , fg" := (Bn_sub d a b (rshift s) fg) (at level 40) : otbn_scope.
+  Notation "'bn.subb' d , a , b , fg" := (Bn_subb d a b (lshift 0) fg) (at level 40) : otbn_scope.
+  Notation "'bn.subb' d , a , b '<<' s , fg" := (Bn_subb d a b (lshift s) fg) (at level 40) : otbn_scope.
+  Notation "'bn.subb' d , a , b '>>' s , fg" := (Bn_subb d a b (rshift s) fg) (at level 40) : otbn_scope.
+  Notation "'bn.movr' a , b" := (Bn_movr a b) (at level 40) : otbn_scope.
+  Notation "'bn.lid' a , offset" := (Bn_lid a offset) (at level 10) : otbn_scope.
+  Notation "'ret'" := Ret (at level 40) : otbn_scope.
+  Notation "'ecall'" := Ecall (at level 40) : otbn_scope.
+  Notation "'jal' a , dst" := (Jal a dst) (at level 40) : otbn_scope.
+  Notation "'bne' a , b , dst" := (Bne a b dst) (at level 40) : otbn_scope.
+  Notation "'beq' a , b , dst" := (Beq a b dst) (at level 40) : otbn_scope.
+  Notation "'loop' a , len" := (Loop a len) (at level 40) : otbn_scope.
+  Notation "'loopi' a , len" := (Loopi a len) (at level 40) : otbn_scope.
+
+  (* Tests for instruction notations. *)
+  Check (addi x3, x0, 5)%otbn.
+  Check (addi x3, x0, -5)%otbn.
+  Check (bn.mulqacc w2.0, w3.3, 64)%otbn.
+  Check (bn.mulqacc.wo.z w4, w2.0, w3.3, 64)%otbn.
+  Check (bn.mulqacc.so w4.L, w2.0, w3.3, 64)%otbn.
+  Check (bn.addm w0, w1, w2)%otbn.
+  Check (bn.subm w0, w1, w2)%otbn.
+  Check (bn.add w0, w0, w0, FG0)%otbn.
+  Check (bn.add w20, w20, w20 << 128, FG0)%otbn.
+  Check (bn.add w20, w20, w20 >> 128, FG1)%otbn.
+  Check (bn.addc w0, w0, w0, FG0)%otbn.
+  Check (bn.addc w20, w20, w20 << 128, FG0)%otbn.
+  Check (bn.addc w20, w20, w20 >> 128, FG1)%otbn.
+  Check (bn.sub w0, w0, w0, FG0)%otbn.
+  Check (bn.sub w20, w20, w20 << 128, FG0)%otbn.
+  Check (bn.sub w20, w20, w20 >> 128, FG1)%otbn.
+  Check (bn.subb w0, w0, w0, FG0)%otbn.
+  Check (bn.subb w20, w20, w20 << 128, FG0)%otbn.
+  Check (bn.subb w20, w20, w20 >> 128, FG1)%otbn.
+  Check (bn.movr x20, x21)%otbn.
+  Check (bn.movr x20++, x21)%otbn.
+  Check (bn.movr x20, x21++)%otbn.
+  Check (bn.lid x20, 0(x21))%otbn.
+  Check (bn.lid x20, 32(x21++))%otbn.
+  Check (bn.lid x20, (-32)(x21++))%otbn.
+  Check (ret)%otbn.
+  Check (ecall)%otbn.
+  Check (bne x3, x4, 0xfde)%otbn.
+  Check (beq x3, x4, 0x400)%otbn.
+  Check (loop x2, 5)%otbn.
+  Check (loopi 2, 5)%otbn.
+End OtbnNotations.
+
+Section ErrorMonad.
+  (* returns either a value or an error message, helpful for debugging *)
+  Definition maybe (A : Type) : Type := A + string.
+  Definition bind {A B} (x : maybe A) (f : A -> maybe B) : maybe B :=
+    match x with
+    | inl a => f a
+    | inr err => inr err
+    end.
+  Definition map_err {A} (x : option A) (err : string) : maybe A :=
+    match x with
+    | Some v => inl v
+    | None => inr err
+    end.
+  Definition prefix_err {A} (x : maybe A) (prefix : string) : maybe A :=
+    match x with
+    | inl v => inl v
+    | inr err => inr (prefix ++ err)%string
+    end.
+  Definition maybe_map {A B} (f : A -> B) (x : maybe A) : maybe B :=
+    match x with
+    | inl v => inl (f v)
+    | inr err => inr err
+    end.
+  Fixpoint maybe_fold_left {A B} (f : A -> B -> maybe A) (l : list B) (x : A) : maybe A :=
+    match l with
+    | [] => inl x
+    | b :: l =>
+        bind (f x b) (maybe_fold_left f l)
+    end.
+  Definition assertion (cond : bool) (msg : string) : maybe unit :=
+    if cond then inl tt else inr msg.
+End ErrorMonad.
+Module ErrorMonadNotations.
+  Notation "a <- b ; c" := (bind b (fun a => c)) (at level 100, right associativity).
+  Notation Ok := inl (only parsing).
+  Notation "'Err' x" := (inr x%string) (at level 20, only parsing).
+End ErrorMonadNotations.
+Import ErrorMonadNotations.
+
+(* Boilerplate definitions for comparing registers. *)
+Section RegisterEquality.
+  Local Ltac derive_eqb r1 r2 :=
+    pose r1 as x1;
+    pose r2 as x2;
+    destruct r1, r2;
+    lazymatch goal with
+    | x1 := ?x, x2 := ?x |- _ => clear; exact true
+    | _ => clear; exact false
+    end.
+  
+  Definition gpr_eqb (r1 r2 : gpr) : bool.
+  Proof. derive_eqb r1 r2. Defined.
+  Definition csr_eqb (r1 r2 : csr) : bool.
+  Proof. derive_eqb r1 r2. Defined.
+  Definition wdr_eqb (r1 r2 : wdr) : bool.
+  Proof. derive_eqb r1 r2. Defined.
+  Definition wsr_eqb (r1 r2 : wsr) : bool.
+  Proof. derive_eqb r1 r2. Defined.
+
+  Local Ltac prove_eqb_spec r1 r2 :=
+    destruct r1, r2; cbv [gpr_eqb]; constructor; congruence.
+  Lemma gpr_eqb_spec : forall r1 r2, BoolSpec (r1 = r2) (r1 <> r2) (gpr_eqb r1 r2).
+  Proof. prove_eqb_spec r1 r2. Qed.
+  Lemma csr_eqb_spec : forall r1 r2, BoolSpec (r1 = r2) (r1 <> r2) (csr_eqb r1 r2).
+  Proof. prove_eqb_spec r1 r2. Qed.
+  Lemma wdr_eqb_spec : forall r1 r2, BoolSpec (r1 = r2) (r1 <> r2) (wdr_eqb r1 r2).
+  Proof. prove_eqb_spec r1 r2. Qed.
+  Lemma wsr_eqb_spec : forall r1 r2, BoolSpec (r1 = r2) (r1 <> r2) (wsr_eqb r1 r2).
+  Proof. prove_eqb_spec r1 r2. Qed.
+End RegisterEquality.
+
+Section FlowGraph.
+  (* control-flow graph of the program *)
+  Inductive ProgramGraph {dst : Type} : Type :=
+  | GraphEcall : ProgramGraph (* ecall instruction *)
+  | GraphLoopEnd : ProgramGraph (* end of loop *)
+  | GraphImemEnd : ProgramGraph (* end of instruction memory -- error *)
+  | GraphStraightline : sinsn -> ProgramGraph -> ProgramGraph (* straightline instruction *)
+  | GraphJump : dst -> ProgramGraph (* jump (may be jal or ret) *)
+  | GraphBne : gpr -> gpr -> dst -> ProgramGraph -> ProgramGraph
+  | GraphBeq : gpr -> gpr -> dst -> ProgramGraph -> ProgramGraph
+  | GraphLoop :
+    (* loop with variable number of iterations *)
+    forall (iters : gpr) (body : ProgramGraph) (post : dst), ProgramGraph
+  | GraphLoopi :
+    (* loop with constant number of iterations *)
+    forall (iters : Z) (body : ProgramGraph) (post : dst), ProgramGraph
   .
 
-  Notation "x ;; 'ecall'" := (Ecall x) (at level 40).
-  Notation "x ;; 'ret'" := (Ret x) (at level 40).
-  Notation "x ;; 'jal' 'x1' , foo ;; y" := (Call x foo y) (at level 60).
-  Notation "x ;; 'jal' 'x0' , foo" := (JumpNoLink x foo) (at level 40).
-  Notation "x ;; 'bne' a , b , foo ;; y" := (Bne x a b foo y) (at level 60).
+  (* traverse the instructions in order, recording only PCs for jumps *)
+  Fixpoint to_graph'
+    (insns : list insn)
+    (curr_pc : Z)
+    (call_stack : list Z)
+    (loop_stack : list Z)
+    : maybe (ProgramGraph (dst:=Z)) :=
+    if ((0 <? length loop_stack)%nat && (curr_pc =? hd 0 loop_stack)%Z)%bool
+    then Ok GraphLoopEnd
+    else
+      match insns with
+      | [] => Ok GraphImemEnd
+      | i :: insns =>
+          match i with
+          | Straightline i =>
+              (post <- to_graph' insns (curr_pc + 4) call_stack loop_stack;
+               Ok (GraphStraightline i post))
+          | Control Ret =>
+              (next_pc <- map_err (hd_error call_stack) "Call stack is empty" ;
+               Ok (GraphJump next_pc))
+          | Control Ecall => Ok GraphEcall
+          | Control (Jal r next_pc) =>
+              (_ <- assertion (gpr_eqb r x1) "Link registers other than x1 are not modelled" ;
+               _ <- assertion (length call_stack <? 8)%nat "Call stack is full" ;
+               post <- to_graph' insns (curr_pc + 4) call_stack loop_stack ;
+               Ok (GraphJump next_pc))
+          | Control (Bne r1 r2 branch_pc) =>
+              (post <- to_graph' insns (curr_pc + 4) call_stack loop_stack ;
+               Ok (GraphBne r1 r2 branch_pc post))
+          | Control (Beq r1 r2 branch_pc) =>
+              (post <- to_graph' insns (curr_pc + 4) call_stack loop_stack ;
+               Ok (GraphBeq r1 r2 branch_pc post))
+          | Control (Loop r len) =>
+              (_ <- assertion (0 <? len) "Loops must have nonzero length" ;
+               _ <- assertion (length loop_stack <? 8)%nat "Loop stack is full" ;
+               let end_pc := curr_pc + 4 * len in
+               body <- to_graph' insns (curr_pc + 4) call_stack (end_pc :: loop_stack) ;
+               Ok (GraphLoop r body end_pc))
+          | Control (Loopi iters len) =>
+              (_ <- assertion (0 <? len) "Loops must have nonzero length" ;
+               _ <- assertion (0 <? iters) "Loopis must have nonzero iterations" ;
+               _ <- assertion (length loop_stack <? 8)%nat "Loop stack is full" ;
+               let end_pc := curr_pc + 4 * len in
+               body <- to_graph' insns (curr_pc + 4) call_stack (end_pc :: loop_stack) ;
+               Ok (GraphLoopi iters body end_pc))
+          end
+      end.
 
-  (* Test notations. *)
-  Check (bn.add w1, w2, w3 << 0, FG0).
-  Check (bn.add w1, w2, w3 >> 3, FG0).
-  Check ([bn.add w1, w2, w3 >> 3, FG0; bn.addm w3, w3, w3] ;; ecall).
-  Check ([bn.add w1, w2, w3 >> 3, FG0; bn.addm w3, w3, w3] ;; jal x1, "foo" ;; [] ;; ret).
-  Check ([bn.add w1, w2, w3 >> 3, FG0; bn.addm w3, w3, w3] ;; jal x0, "foo").
-  Check ([bn.add w1, w2, w3 >> 3, FG0; bn.addm w3, w3, w3] ;; bne x1, x2, "foo" ;; [] ;; ret).
+  Fixpoint get_dst_pcs (g : ProgramGraph (dst:=Z)) : list Z :=
+    match g with
+    | GraphEcall | GraphLoopEnd | GraphImemEnd => []
+    | GraphStraightline i g => get_dst_pcs g
+    | GraphJump pc => [pc]
+    | GraphBne r1 r2 pc g => pc :: get_dst_pcs g
+    | GraphBeq r1 r2 pc g => pc :: get_dst_pcs g
+    | GraphLoop r body pc => pc :: get_dst_pcs body
+    | GraphLoopi iters body pc => pc :: get_dst_pcs body
+    end.
+
+  (* for each PC, if there is a jump to that PC or if the PC is the
+     start PC, then construct the program graph that flows from it *)
+  (*
+  Definition to_graph (insns : list insn) : maybe (ProgramGraph (dst:=ProgramGraph)) :=
    *)
-End Notations.
 
-(* error monad : either a value or an error message *)
-Definition maybe (A : Type) : Type := A + string.
-Definition bind {A B} (x : maybe A) (f : A -> maybe B) : maybe B :=
-  match x with
-  | inl a => f a
-  | inr err => inr err
-  end.
-Definition map_err {A} (x : option A) (err : string) : maybe A :=
-  match x with
-  | Some v => inl v
-  | None => inr err
-  end.
-Definition prefix_err {A} (x : maybe A) (prefix : string) : maybe A :=
-  match x with
-  | inl v => inl v
-  | inr err => inr (prefix ++ err)%string
-  end.
-Definition maybe_map {A B} (f : A -> B) (x : maybe A) : maybe B :=
-  match x with
-  | inl v => inl (f v)
-  | inr err => inr err
-  end.
-Definition assertion (cond : bool) (msg : string) : maybe unit :=
-  if cond then inl tt else inr msg.
-Local Notation "a <- b ; c" := (bind b (fun a => c)) (at level 100, right associativity).
-Local Notation "'assert!' x msg" := (if x then inr msg%string else inl tt) (at level 40).
-Local Notation Ok := inl (only parsing).
-Local Notation Err := inr (only parsing).
+End FlowGraph.
 
 (* bitwise operation shorthand *)
 Local Infix "|'" := Z.lor (at level 40, only parsing) : Z_scope.
@@ -209,20 +397,23 @@ Section Exec.
     {mget_mset_neq : forall K V (m : map K V) k1 k2 v,
         k1 <> k2 -> mget (mset m k1 v) k2 = mget m k2}.
   Arguments mget {_ _}. Arguments mset {_ _}.
+  Notation regfile := (map reg Z) (only parsing).
+  Notation flagfile := (map flag bool) (only parsing).
+  Notation mem := (map Z Z) (only parsing).
 
   (* State information for the processor. *)
   Record OtbnState : Type :=
     {
       (* Register file. *)
-      regfile : map reg Z;
+      regs : regfile;
       (* Flag states. *)
-      flagfile : map flag bool;
+      flags : flagfile;
       (* Data memory *)
-      dmem : map Z Z;
-      (* Call stack. *)
+      dmem : mem;
+      (* Call stack: holds the IMEM address of the last calls. *)
       callstack : list Z;
-      (* Loop stack; holds the number of iterations remaining for each loop. *)
-      loopstack : list Z;
+      (* Loop stack: holds the IMEM start/end addresses and counter for active loops. *)
+      loopstack : list (Z * Z * nat);
       (* Instruction counter. *)
       insn_counter : nat;
     }.
@@ -233,22 +424,22 @@ Section Exec.
     | x1 =>
         (* TODO: a direct read from the call stack is possible but
            rare in practice. For now, don't model it. *)
-        Err "Attempt to directly read from the call stack. This behavior is not yet modelled."%string
-    | _ => map_err (mget st.(regfile) (gpreg r)) "GPR undefined"
+        Err "Attempt to directly read from the call stack. This behavior is not yet modelled."
+    | _ => map_err (mget st.(regs) (gpreg r)) "GPR undefined"
     end.
 
   Definition read_wdr (st : OtbnState) (r : wdr) : maybe Z :=
-    map_err (mget st.(regfile) (wdreg r)) "WDR undefined".
+    map_err (mget st.(regs) (wdreg r)) "WDR undefined".
 
   Definition read_wsr (st : OtbnState) (r : wsr) : maybe Z :=
     match r with
     | RND => Ok (rnd (st.(insn_counter)))
     | URND => Ok (urnd st.(insn_counter))
-    | _ => map_err (mget st.(regfile) (wsreg r)) "WSR undefined"
+    | _ => map_err (mget st.(regs) (wsreg r)) "WSR undefined"
     end.
 
   Definition read_flag (st : OtbnState) (f : flag) : maybe bool :=
-    map_err (mget st.(flagfile) f) "Flag undefined".
+    map_err (mget st.(flags) f) "Flag undefined".
 
   (* Assemble a group of flags into an integer value. *)
   Definition read_flag_group (st : OtbnState) (fg : flag_group) : maybe Z :=
@@ -286,8 +477,8 @@ Section Exec.
   end.
 
   Definition inc_insn_counter (st : OtbnState) : OtbnState :=
-    {| regfile := st.(regfile);
-      flagfile := st.(flagfile);
+    {| regs := st.(regs);
+      flags := st.(flags);
       dmem := st.(dmem);
       callstack := st.(callstack);
       loopstack := st.(loopstack);
@@ -295,13 +486,29 @@ Section Exec.
     |}.
 
   Definition regfile_set (st : OtbnState) (r : reg) (v : Z) : OtbnState :=
-    {| regfile := mset st.(regfile) r v;
-      flagfile := st.(flagfile);
+    {| regs := mset st.(regs) r v;
+      flags := st.(flags);
       dmem := st.(dmem);
       callstack := st.(callstack);
       loopstack := st.(loopstack);
       insn_counter := st.(insn_counter);
     |}.
+
+  Definition flagfile_set (st : OtbnState) (f : flag) (v : bool) : OtbnState :=
+    {| regs := st.(regs);
+      flags := mset st.(flags) f v;
+      dmem := st.(dmem);
+      callstack := st.(callstack);
+      loopstack := st.(loopstack);
+      insn_counter := st.(insn_counter);
+    |}.
+
+  (* set the M, L, and Z flags according to the destination register *)
+  Definition set_mlz (st : OtbnState) (fg : flag_group) (v : Z) : OtbnState :=
+    let st := flagfile_set st (flagM fg) (Z.testbit v 255) in
+    let st := flagfile_set st (flagL fg) (Z.testbit v 0) in
+    let st := flagfile_set st (flagZ fg) (v =? 0) in
+    st.
 
   Definition cast32 (v : Z) : Z := v &' Z.ones 32.
   Definition cast256 (v : Z) : Z := v &' Z.ones 256.
@@ -313,7 +520,7 @@ Section Exec.
         (* TODO: this should push to the call stack, but is
            practically never used. For now, don't model this behavior
            and treat it as an error. *)
-        Err "Attempt to write to call stack. This behavior is not yet modelled."%string
+        Err "Attempt to write to call stack. This behavior is not yet modelled."
     | _ => Ok (regfile_set st (gpreg r) (cast32 v))
     end.
 
@@ -328,26 +535,341 @@ Section Exec.
 
   (* mulqacc shifts must be multiples of 64 *)
   Definition valid_mul_shift (s : Z) : bool :=
-    ((s =? 0)%Z || (s =? 64)%Z || (s =? 128%Z) || (s =? 192%Z))%bool.
+    ((s =? 0) || (s =? 64) || (s =? 128) || (s =? 192)).
+  (* rshi shifts must be in the range [0,255] *)
+  Definition valid_rshi_imm (s : Z) : bool :=
+    (0 <=? s) && (s <? 256).
   (* other shift immediates must be multiples of 8 and in the range [0,248] *)
   Definition valid_arith_shift (s : shift) : bool :=
     let s := match s with
              | lshift x => x
              | rshift x => x
              end in
-    ((s mod 8 =? 0)%Z && (0 <=? s)%Z && (s <=? 248)%Z)%bool.
+    ((s mod 8 =? 0) && (0 <=? s) && (s <=? 248)).
+  (* immediates for addi must be in the range [-2048, 2047] *)
+  Definition valid_addi_imm (imm : Z) : bool :=
+    (-2048 <=? imm) && (imm <=? 2047).
+  (* offsets for loads and stores are in the range [-16384, 16352] in steps of 32 *)
+  Definition valid_mem_offset (offset : Z) : bool :=
+    (-16384 <=? offset) && (offset <=? 16352) && (offset mod 32 =? 0).
 
+  (* returns whether the indirect register should be incremented *)
+  Definition has_inc (x : ind) : bool :=
+    match x with
+    | ind_noinc r => false
+    | ind_inc r => true
+    end.
+  (* gets the gpr corresponding to this indirect value *)
+  Definition ind_to_gpr (x : ind) : gpr :=
+    match x with
+    | ind_noinc r => r
+    | ind_inc r => r
+    end.
+  (* get a wdr by its index value *)
+  Definition index_to_wdr (idx : Z) : maybe wdr :=
+    match idx with
+    | 0 => Ok w0
+    | 1 => Ok w1
+    | 2 => Ok w2
+    | 3 => Ok w3
+    | 4 => Ok w4
+    | 5 => Ok w5
+    | 6 => Ok w6
+    | 7 => Ok w7
+    | 8 => Ok w8
+    | 9 => Ok w9
+    | 10 => Ok w10
+    | 11 => Ok w11
+    | 12 => Ok w12
+    | 13 => Ok w13
+    | 14 => Ok w14
+    | 15 => Ok w15
+    | 16 => Ok w16
+    | 17 => Ok w17
+    | 18 => Ok w18
+    | 19 => Ok w19
+    | 20 => Ok w20
+    | 21 => Ok w21
+    | 22 => Ok w22
+    | 23 => Ok w23
+    | 24 => Ok w24
+    | 25 => Ok w25
+    | 26 => Ok w26
+    | 27 => Ok w27
+    | 28 => Ok w28
+    | 29 => Ok w29
+    | 30 => Ok w30
+    | 31 => Ok w31
+    | _ => Err "Invalid WDR index"
+    end.
+  (* gets the value from the wdr corresponding to this indirect value *)
+  Definition read_ind (st : OtbnState) (x : ind) : maybe Z :=
+    let r := ind_to_gpr x in
+    ptr <- read_gpr st r ;
+    w <- index_to_wdr (ptr &' 32) ;
+    read_wdr st w.
+
+  (* specifications for complex operations (may make proofs a little nicer) *)
+  Definition mulqacc_spec (acc x y s : Z) : Z :=
+    acc + (x * y) << s.
   Definition addm_spec (x y m : Z) : Z :=
     let r := x + y in
     if r >? m then r - m else r.
   Definition subm_spec (x y m : Z) : Z :=
     let r := x - y in
     if r <? 0 then r + m else r.
+  Definition rshi_spec (x y imm : Z) : Z :=
+    let xy := Z.lor (x << 256) y in
+    xy >> imm.
 
   Definition exec1
-    (st : OtbnState) (i : Insn) : maybe OtbnState :=
+    (st : OtbnState) (i : sinsn) : maybe OtbnState :=
+    match i with
+    | Addi d x imm =>
+        (_ <- assertion (valid_addi_imm imm) "Invalid immediate for addi";
+         x <- read_gpr st x ;
+         write_gpr st d (x + imm))
+    | Bn_mulqacc z x y s =>
+        let st := if z then write_wsr st ACC 0 else st in
+        (_ <- assertion (valid_mul_shift s) "Invalid shift for bn.mulqacc";
+         x <- read_limb st x ;
+         y <- read_limb st y ;
+         acc <- read_wsr st ACC ;
+         let r := mulqacc_spec acc x y s in
+         Ok (write_wsr st ACC r))
+    | Bn_mulqacc_wo z d x y s =>
+        let st := if z then write_wsr st ACC 0 else st in
+        (_ <- assertion (valid_mul_shift s) "Invalid shift for bn.mulqacc.wo" ;
+         x <- read_limb st x ;
+         y <- read_limb st y ;
+         acc <- read_wsr st ACC ;
+         let r := mulqacc_spec acc x y s in
+         Ok (write_wdr (write_wsr st ACC r) d r))
+    | Bn_mulqacc_so z L d x y s =>
+        let st := if z then write_wsr st ACC 0 else st in
+        (_ <- assertion (valid_mul_shift s) "Invalid shift for bn.mulqacc.so" ;
+         x <- read_limb st x ;
+         y <- read_limb st y ;
+         old <- read_wdr st d ;
+         acc <- read_wsr st ACC ;
+         let r := mulqacc_spec acc x y s in
+         let accL := r &' (Z.ones 128) in
+         let accH := r >> 128 in
+         let dL := old &' (Z.ones 128) in
+         let dH := old >> 128 in
+         let d' := if L
+                   then (accL |' (dH << 128))
+                   else (dL |' (accL << 128)) in
+         Ok (write_wdr (write_wsr st ACC r) d d'))
+    | Bn_addm d x y =>
+         (x <- read_wdr st x ;
+          y <- read_wdr st y ;
+          m <- read_wsr st MOD ;          
+          Ok (write_wdr st d (addm_spec x y m)))
+    | Bn_subm d x y =>
+         (x <- read_wdr st x ;
+          y <- read_wdr st y ;
+          m <- read_wsr st MOD ;
+          Ok (write_wdr st d (subm_spec x y m)))
+    | Bn_add d x y s fg =>
+        (_ <- assertion (valid_arith_shift s) "Invalid shift for bn.add" ;
+         x <- read_wdr st x ;
+         y <- read_wdr st y ;
+         let r := x + y in
+         let st := set_mlz st fg r in
+         let st := flagfile_set st (flagC fg) (2^256 <=? r) in
+         Ok (write_wdr st d r))
+    | Bn_addc d x y s fg =>
+        (_ <- assertion (valid_arith_shift s) "Invalid shift for bn.addc" ;
+         c <- read_flag st (flagC fg);
+         x <- read_wdr st x ;
+         y <- read_wdr st y ;
+         let r := x + y + c in
+         let st := set_mlz st fg r in
+         let st := flagfile_set st (flagC fg) (2^256 <=? r) in
+         Ok (write_wdr st d r))
+    | Bn_sub d x y s fg =>
+        (_ <- assertion (valid_arith_shift s) "Invalid shift for bn.sub" ;
+         x <- read_wdr st x ;
+         y <- read_wdr st y ;
+         let r := x - y in
+         let st := set_mlz st fg r in
+         let st := flagfile_set st (flagC fg) (r <? 0) in
+         Ok (write_wdr st d r))
+    | Bn_subb d x y s fg =>
+        (_ <- assertion (valid_arith_shift s) "Invalid shift for bn.subb" ;
+         b <- read_flag st (flagC fg);
+         x <- read_wdr st x ;
+         y <- read_wdr st y ;
+         let r := x - y - b in
+         let st := set_mlz st fg r in
+         let st := flagfile_set st (flagC fg) (r <? 0) in
+         Ok (write_wdr st d r))
+    | Bn_rshi d x y imm =>
+        (_ <- assertion (valid_rshi_imm imm) "Invalid immediate for bn.rshi" ;
+         x <- read_wdr st x ;
+         y <- read_wdr st y ;
+         let r := rshi_spec x y imm in
+         Ok (write_wdr st d r))
+    | Bn_movr x y =>
+        let xinc := has_inc x in
+        let yinc := has_inc y in
+        let xr := ind_to_gpr x in
+        let yr := ind_to_gpr y in
+        (_ <- assertion (negb(xinc && yinc)) "Cannot increment both indirect registers (bn.movr)";
+         src_ptr <- read_gpr st yr ;
+         src <- index_to_wdr (src_ptr &' 32) ;
+         dst_ptr <- read_gpr st xr ;
+         dst <- index_to_wdr (dst_ptr &' 32) ;
+         v <- read_wdr st src ;
+         st <- (if xinc
+                then write_gpr st xr (src_ptr + 1)
+                else if yinc
+                     then write_gpr st yr (dst_ptr + 1)
+                     else Ok st) ;
+         Ok (write_wdr st dst v))
+    | Bn_lid x offset y =>
+        let xinc := has_inc x in
+        let yinc := has_inc y in
+        let xr := ind_to_gpr x in
+        let yr := ind_to_gpr y in
+        (_ <- assertion (negb(xinc && yinc)) "Cannot increment both indirect registers (bn.lid)";
+         _ <- assertion (valid_mem_offset offset) "Invalid offset for bn.lid";
+         src_ptr <- read_gpr st yr ;
+         src <- index_to_wdr (src_ptr &' 32) ;
+         dst_ptr <- read_gpr st xr ;
+         dst <- index_to_wdr (dst_ptr &' 32) ;
+         v <- read_wdr st src ;
+         st <- (if xinc
+                then write_gpr st xr (src_ptr + 1)
+                else if yinc
+                     then write_gpr st yr (dst_ptr + 1)
+                     else Ok st) ;
+         Ok (write_wdr st dst v))
+          (*
+    | _ => Err "NotImplemented"
+*)
+    end.
+
+  Definition exec_straightline
+    (st : OtbnState) (insns : list sinsn) : maybe OtbnState :=
+    fold_left (fun st i => (st <- st ;
+                            st <- exec1 st i;
+                            Ok (inc_insn_counter st)))
+      insns (Ok st).
+
+  Definition exec_straightline_cps {A}
+    (st : OtbnState) (insns : list sinsn) (f : maybe OtbnState -> A) : A :=
+    f (exec_straightline st insns).
+
+  (* Test *)
+  Import OtbnNotations.
+  Goal (forall st,
+           read_wdr st w2 = Ok 5 ->
+           (st <- exec_straightline st
+                    [(addi x2, x0, 2)%otbn;
+                     (bn.add w0, w2, w2, FG0)%otbn];
+            read_wdr st w0) = Ok 10).
+  Proof.
+    intros; cbn. destruct st.
+    cbv [read_wdr inc_insn_counter regs prefix_err] in *; cbn.
+    rewrite !mget_mset_neq by congruence.
+    lazymatch goal with
+    | H : _ = inl _ |- _ => rewrite H; cbn [bind]
+    end.
+    cbn [write_wdr regfile_set regs].
+    rewrite ?mget_mset_neq by congruence.
+    rewrite mget_mset_eq by congruence.
+    reflexivity.
+  Qed.
+
+  Print cinsn.
+  Print OtbnState.
+  Definition ctrl1 (pc_st : Z * OtbnState) (i : cinsn) : maybe (Z * OtbnState) :=
+    let pc := fst pc_st in
+    let st := snd pc_st in
+    
+    match cinsn with
+    | Ret =>
+        (next_pc <- map_err (hd_error st.(callstack) "Call stack is empty" ;
+         Ok (GraphJump next_pc))
+          | Control Ecall => Ok GraphEcall
+          | Control (Jal r next_pc) =>
+              (_ <- assertion (gpr_eqb r x1) "Link registers other than x1 are not modelled" ;
+               _ <- assertion (length call_stack <? 8)%nat "Call stack is full" ;
+               post <- to_graph' insns (curr_pc + 4) call_stack loop_stack ;
+               Ok (GraphJump next_pc))
+          | Control (Bne r1 r2 branch_pc) =>
+              (post <- to_graph' insns (curr_pc + 4) call_stack loop_stack ;
+               Ok (GraphBne r1 r2 branch_pc post))
+          | Control (Beq r1 r2 branch_pc) =>
+              (post <- to_graph' insns (curr_pc + 4) call_stack loop_stack ;
+               Ok (GraphBeq r1 r2 branch_pc post))
+          | Control (Loop r len) =>
+              (_ <- assertion (0 <? len) "Loops must have nonzero length" ;
+               _ <- assertion (length loop_stack <? 8)%nat "Loop stack is full" ;
+               let end_pc := curr_pc + 4 * len in
+               body <- to_graph' insns (curr_pc + 4) call_stack (end_pc :: loop_stack) ;
+               Ok (GraphLoop r body end_pc))
+          | Control (Loopi iters len) =>
+              (_ <- assertion (0 <? len) "Loops must have nonzero length" ;
+               _ <- assertion (0 <? iters) "Loopis must have nonzero iterations" ;
+               _ <- assertion (length loop_stack <? 8)%nat "Loop stack is full" ;
+               let end_pc := curr_pc + 4 * len in
+               body <- to_graph' insns (curr_pc + 4) call_stack (end_pc :: loop_stack) ;
+               Ok (GraphLoopi iters body end_pc))
+          end
+
+  Section __.
+    Context (blocks : map Z (list sinsn * cinsn)).
+    
+    Print cinsn.
+    Inductive exec : string -> OtbnState -> (option string -> OtbnState -> Prop) -> Prop :=
+    | ExecBlock lbl st post
+        sis ci (_:mget blocks lbl = Some (sis, ci))
+        f (_:exec_straightline_cps st sis (fun st => post) = )
+      :
+      exec_straightline_cps st 
+      
+    .
+  End __.
+
+  Fixpoint exec
+    (labels : map string Z)
+    (blocks : map Z Block)
+    (st : OtbnState)
+    (start : Block) : maybe OtbnState :=
+    match start with
+    | Ret insns =>
+        (st <- exec_straightline st insns ;
+         pc <- map_err (hd_error st.(callstack)) "Call stack empty" ;
+         b <- map_err (mget blocks pc) "No block found for PC";
+         exec labels blocks st b)
+    | _ => Err "NotImplemented"
+    end.
+  
+
+  Definition run1
+    (i : sinsn)
+    (regs : regfile) (flags : flagfile) (dmem : mem)
+    (P : regfile -> flagfile -> mem -> Prop)
+    : Prop :=
     match i with
     | Mulqacc z x y s =>
+        exists vx vy vacc,
+        read_limb regs x = Ok vx
+        /\ read_limb regs y = Ok vy
+        /\ read_wsr regs ACC = Ok vacc
+        /\ valid_mul_shift s
+        /\ (let x := vx in
+            let y := vy in
+            let acc := vacc in
+            let r := (acc + ((x * y) << s)) in
+            let regs' := write_wsr regs ACC r in
+            P regs' flags dmem)
+    end.
+
+        
         let st := if z then write_wsr st ACC 0 else st in
         (_ <- assertion (valid_mul_shift s) "Invalid shift for bn.mulqacc" ;
          x <- read_limb st x ;
@@ -394,27 +916,9 @@ Section Exec.
          x <- read_wdr st x ;
          y <- read_wdr st y ;
          Ok (write_wdr st d (x + y + c)))
-    | _ => Err "NotImplemented"%string
+    | _ => Err "NotImplemented"
     end.
 
-  Definition exec_straightline
-    (st : OtbnState) (insns : list Insn) : maybe OtbnState :=
-    fold_left (fun st i => (st <- st;
-                            st <- exec1 st i;
-                            Ok (inc_insn_counter st))) insns (Ok st).    
-
-  Print Block.
-  Fixpoint exec
-    (labels : map string Block) (st : OtbnState) (start : Block) : maybe OtbnState :=
-    match start with
-    | Ret insns =>
-        (st <- exec_straightline st insns ;
-         loc <- map_err (hd_error st.(callstack)) "Call stack empty"%string ;
-         exec labels st loc)
-    | _ => Err "NotImplemented"%string
-    end.
-
-  
 
   
 End Exec.
